\lecture{33}{2021-11-22}{}

\begin{thm}{Algebraic Manipulation of Derivatives}{}
	If \(f \colon A \subset \mathbb{R} \to \mathbb{R}\), \(g \colon A \subset \mathbb{R} \to \mathbb{R}\), and \(f'(c)\), \(g'(c)\) exist, then:
	\begin{enumerate}
		\item \((f+g)'(c) = f'(c) + g'(c)\);
		\item \((kf)'(c) = kf'(c)\);
		\item \((fg)'(c) = f'(c)g(c) + f(c)g'(c)\)
		\item \((f/g)'(c) = \frac{f'(c)g(c) - f(c)g'(c)}{g(c)^2}\), if \(g(c) \neq 0\).
	\end{enumerate}
\end{thm}

\begin{dem}{}{}
	\begin{enumerate}
		\item \textcolor{red}{To be done.}
		\item \textcolor{red}{To be done.}
		\item Note that
			\begin{align*}
				(fg)'(c) &= \lim_{x \to c} \frac{f(x)g(x) - f(c)g(c)}{x-c} \\
						 &= \lim_{x \to c} \frac{f(x)g(x) - f(x)g(c) + f(x)g(c) - f(c)g(c)}{x-c} \\
						 &= \lim_{x \to c} \frac{f(x)(g(x) - g(c)) + (f(x) - f(c))g(c)}{x-c} \\
						 &= \lim_{x \to c} \frac{f(x)(g(x) - g(c))}{x - c} + \lim_{x \to c} \frac{(f(x) - f(c))g(c)}{x-c} \\
						 &= f(c)g'(c) + f'(c)g(c).
			\end{align*}
		\item \textcolor{red}{To be done.}
	\end{enumerate}
\end{dem}
